removed extended language constructs

thorin/semantics_full/lang.v
@@ -49,6 +49,7 @@ but by construction, T is normalized
   - 'beta reduce until norm' does not really hold (and if so only if not under binder)
 - TODO: there should not be any type reduxes (except maybe toplevel?)
   - no redex in the type of a lambda
+  - same with sigma
   - can Pi have a redex => should have, right?
 
 
@@ -86,8 +87,9 @@ Outline types_sol.v:
 
 
 Inductive expr :=
-  | Star
-  | Box
+  (* | Star
+  | Box *)
+  | Sort (n:nat)
   | Bot
   | Nat
   | Idx 
@@ -100,11 +102,11 @@ Inductive expr :=
   (* lam has a filter expression *)
   | Lam (x : binder) (T : expr) (f : expr) (U: expr) (e: expr)
   | App (e1 e2 : expr)
-  (* | Sigma (args: list (binder * expr))
+  | Sigma (args: list (binder * expr))
   | Tuple (es : list expr)
   | Array (x: binder) (en: expr) (T: expr)
   | Pack (x: binder) (en: expr) (e: expr)
-  | Extract (e: expr) (ei: expr) *)
+  | Extract (e: expr) (ei: expr)
 .
 
 Bind Scope expr_scope with expr.
@@ -133,44 +135,10 @@ Bind Scope expr_scope with expr.
   All our proofs only argue about is_val.
 *)
 
-Inductive is_val : expr → Prop :=
-  | StarV : is_val Star
-  | BoxV : is_val Box
-  | BotV : is_val Bot
-  | NatV : is_val Nat
-  | IdxV : is_val Idx
-  (* TODO: is (Idx n) a value? if not what does it reduce to *)
-  | IdxAppV n : is_val (App Idx (LitNat n))
-  | LitNatV n : is_val (LitNat n)
-  | LitIdxV n i : is_val (LitIdx n i)
-  | PiV x T U : 
-    is_val T →
-    is_val (Pi x T U)
-  | LamV x T f U e : 
-    is_val T →
-    (* U might depend on x:T *)
-    is_val (Lam x T f U e)
-  (* compound values *)
-  (* 
-    sigma is like lambda (functions depending on previous values)
-    => only the first one should be a val
-  *)
-  (* | SigmaEmptyV: is_val (Sigma [])
-  (* we do not need to test the rest => (implicitely) depends on first one *)
-  | SigmaConsV x T args : is_val T → is_val (Sigma ((x, T) :: args))
-  | TupleV es : Forall is_val es → is_val (Tuple es)
-  | ArrayV x en T : 
-    is_val en →
-    is_val (Array x en T)
-  | PackV x en e :
-    is_val en →
-    is_val (Pack x en e) *)
-  .
-
 Fixpoint subst (x : string) (es : expr) (e : expr)  : expr :=
   let recurse_under y expr := if decide (y = BNamed x) then expr else subst x es expr in
   match e with
-  | Star | Box | Bot | Nat | Idx | LitNat _ | LitIdx _ _  => e
+  | Sort _ | Bot | Nat | Idx | LitNat _ | LitIdx _ _  => e
   | Var y => if decide (y = x) then es else e
   (* replace x in T, replace in U if not x *)
   | Pi y T U => 
@@ -187,7 +155,7 @@ Fixpoint subst (x : string) (es : expr) (e : expr)  : expr :=
   mutual recursion is not recognized (https://coq.discourse.group/t/mutual-recursion-for-nested-inductive-types/729/3)
   Equations would be possible but not necessarily easier
    *)
-  (* | Tuple expression =>
+  | Tuple expression =>
     Tuple (map (subst x es) expression)
   (* for Sigma, we only continue subst in args if not already encountered var *)
   | Sigma xs =>
@@ -200,7 +168,7 @@ Fixpoint subst (x : string) (es : expr) (e : expr)  : expr :=
       end) xs)
   | Array y en T => Array y (subst x es en) (recurse_under y T)
   | Pack y en e => Pack y (subst x es en) (recurse_under y e)
-  | Extract e ei => Extract (subst x es e) (subst x es ei) *)
+  | Extract e ei => Extract (subst x es e) (subst x es ei)
   end.
 
 Definition subst' (mx : binder) (es : expr) : expr → expr :=
@@ -280,13 +248,14 @@ Definition ETrue := LitIdx 2 (Fin.FS Fin.F1).
 (* TODO: require normalized subexpressions? (would be needed for in-to-out-order) *)
 Inductive normalize_step : expr -> expr -> Prop :=
   (* no let *)
-  (* | normalize_extract_one e:
+  | normalize_extract_one e:
     (* TODO: need normalized of e? *)
     normalize_step (Extract e (LitIdx 1 Fin.F1)) e
   | normalize_tuple_one e:
     normalize_step (Tuple [e]) e
-  | normalize_sigma_one xT:
-    normalize_step (Sigma [xT]) (Sigma [xT])
+  | normalize_sigma_one x T:
+    normalize_step (Sigma [(x,T)]) T
+    (* normalize_step (Sigma [xT]) (Sigma [xT]) *)
   | normalize_tuple_beta xs n i e:
     length xs = n ->
     nth_error xs (` (Fin.to_nat i)) = Some e ->
@@ -304,15 +273,21 @@ Inductive normalize_step : expr -> expr -> Prop :=
     normalize_step (Tuple (replicate n e)) (Pack (BAnon) (LitNat n) e)
   | normalize_array_sigma n T:
     n > 1 ->
-    normalize_step (Sigma (replicate n (BAnon, T))) (Array (BAnon) (LitNat n) T) *)
+    normalize_step (Sigma (replicate n (BAnon, T))) (Array (BAnon) (LitNat n) T)
   | normalize_beta x T ef U eb ea:
     (* TODO: ef[ea/x] beta equiv true *)
     ef = ETrue ->
     normalize_step (App (Lam x T ef U eb) ea) (subst' x ea eb)
-  (* | normalize_tuple_pack x n e:
+  | normalize_tuple_pack x n e:
     normalize_step (Pack (BNamed x) (LitNat n) e) (Tuple (instantiate x n e))
   | normalize_sigma_array x n T:
-    normalize_step (Array (BNamed x) (LitNat n) T) (Sigma (map (fun x => (BAnon, x)) (instantiate x n T))) *)
+    normalize_step (Array (BNamed x) (LitNat n) T) (Sigma (map (fun x => (BAnon, x)) (instantiate x n T)))
+
+  (* TODO: not in paper *)
+  | normalize_pack_one e:
+    normalize_step (Pack BAnon (LitNat 1) e) e
+  | normalize_array_one T:
+    normalize_step (Array BAnon (LitNat 1) T) T
 .
 
 (* TODO: do we need to require left-to-right or in-to-out order? *)
@@ -326,14 +301,14 @@ Inductive full_ectx :=
   | FLam4 (x:binder) (T: expr) (f:expr) (U:expr) (e:full_ectx)
   | FApp1 (K: full_ectx) (e2 : expr)
   | FApp2 (e1 : expr) (K: full_ectx)
-  (* | FSigma (xs1: list (binder * expr)) (x:binder) (K: full_ectx) (xs2: list (binder * expr))
+  | FSigma (xs1: list (binder * expr)) (x:binder) (K: full_ectx) (xs2: list (binder * expr))
   | FTuple (es1:list expr) (K: full_ectx) (es2: list expr)
   | FArray1 (x:binder) (en: full_ectx) (T:expr)
   | FArray2 (x:binder) (en: expr) (T: full_ectx)
   | FPack1 (x:binder) (en: full_ectx) (e:expr)
   | FPack2 (x:binder) (en: expr) (e: full_ectx)
   | FExtract1 (K: full_ectx) (ei:expr)
-  | FExtract2 (e:expr) (K: full_ectx) *)
+  | FExtract2 (e:expr) (K: full_ectx)
   .
 
 Fixpoint full_fill (K:full_ectx) (e:expr) : expr :=
@@ -347,14 +322,14 @@ Fixpoint full_fill (K:full_ectx) (e:expr) : expr :=
   | FLam4 x T f U K  => Lam x T f U (full_fill K e)
   | FApp1 K e2 => App (full_fill K e) e2
   | FApp2 e1 K => App e1 (full_fill K e)
-  (* | FSigma xs1 x K xs2 => Sigma (xs1 ++ (x,full_fill K e) :: xs2)
+  | FSigma xs1 x K xs2 => Sigma (xs1 ++ (x,full_fill K e) :: xs2)
   | FTuple es1 K es2 => Tuple (es1 ++ full_fill K e :: es2)
   | FArray1 x K T => Array x (full_fill K e) T
   | FArray2 x en K => Array x en (full_fill K e)
   | FPack1 x K eb => Pack x (full_fill K e) eb
   | FPack2 x en K => Pack x en (full_fill K e)
   | FExtract1 K ei => Extract (full_fill K e) ei
-  | FExtract2 eb K => Extract eb (full_fill K e) *)
+  | FExtract2 eb K => Extract eb (full_fill K e)
   end.
 
 Inductive full_contextual_step (e1 : expr) (e2 : expr) : Prop :=
@@ -376,13 +351,17 @@ Definition normal_eval e e' :=
 (*
   a bit more constructive version
   => subexpressions and contradict normalization step in negative assumptions
+
+
+  TODO: change
 *)
 Inductive normalized : expr -> Prop :=
   (* atomic values *)
   (* conceptually, every value is normalized (not quite -- normalization goes under binders) *)
   (* but for distinction, differences and adaptation, we should keep normalization without is_val *)
-  | norm_Star: normalized Star
-  | norm_Box: normalized Box
+  (* | norm_Star: normalized Star
+  | norm_Box: normalized Box *)
+  | norm_Sort n: normalized (Sort n)
   | norm_Bot: normalized Bot
   | norm_Nat: normalized Nat
   | norm_Idx: normalized Idx
@@ -410,7 +389,7 @@ Inductive normalized : expr -> Prop :=
     - not unary
     - no unnamed array sigma [T, ..., T]
   *)
-  (* | norm_Sigma xs:
+  | norm_Sigma xs:
     (* without map separately, it would be a not strictly positive occurence of normalized *)
     Forall normalized (map (fun '(x,T) => T) xs) ->
     xs = [] \/ length xs > 1 ->
@@ -466,10 +445,72 @@ Inductive normalized : expr -> Prop :=
     ~ (ei = LitIdx 1 Fin.F1) ->
     ~ (exists es idx, e = Tuple es /\ ei = LitIdx (length es) idx) ->
     ~ (exists en eb, e = Pack BAnon en eb) ->
-    normalized (Extract e ei) *)
+    normalized (Extract e ei)
+  .
+(* TODO:
+  enumerate full constructive (as far as possible) normalized predicate
+  TODO: not up to date
+
+
+  we define is_val for normalized expressions => does not contain a beta redex
+  we do not go into types of dependencies (only decent along evaluation contexts)
+  but we descend under binders
+
+  applications and extracts are not values
+*)
+Inductive is_val : expr → Prop :=
+(* with is_val : expr → Prop := *)
+  (* atomic values *)
+  (* | StarV : is_val Star
+  | BoxV : is_val Box *)
+  | SortV n : is_val (Sort n)
+  | BotV : is_val Bot
+  | NatV : is_val Nat
+  | IdxV : is_val Idx
+  (* TODO: is (Idx n) a value? if not what does it reduce to *)
+  | IdxAppV n : is_val (App Idx (LitNat n))
+  | LitNatV n : is_val (LitNat n)
+  | LitIdxV n i : is_val (LitIdx n i)
+  | PiV x T U : 
+    (* is_val T → *)
+    is_val (Pi x T U)
+  | LamV x T f U e : 
+    (* TODO: should this be value or normalized?
+    => we step not in the type
+    => normalization already sufficient for value
+     *)
+    (* is_val T → *)
+    (* normalized T → *)
+    (* U might depend on x:T *)
+    is_val e ->
+    is_val (Lam x T f U e)
+  (* compound values *)
+  (* 
+    sigma is like lambda (functions depending on previous values)
+    => only the first one should be a val
+  *)
+  | SigmaV xs: is_val (Sigma xs)
+  (* | SigmaEmptyV: is_val (Sigma [])
+  (* we do not need to test the rest => (implicitely) depends on first one *)
+  | SigmaConsV x T args : 
+    (* same as lambda *)
+    (* is_val T →  *)
+    (* normalized T → *)
+    is_val (Sigma ((x, T) :: args)) *)
+  | TupleV es : Forall is_val es → is_val (Tuple es)
+  | ArrayV x en T : 
+    (* is_val en →
+    is_val T → *)
+    is_val (Array x en T)
+  | PackV x en e :
+    is_val en →
+    is_val e →
+    is_val (Pack x en e)
   .
 
-Lemma normalized_sound e:
+
+
+(* Lemma normalized_sound e:
   (* normalized_pred := ~ normalizable *)
   normalized e -> ~ normalizable e.
 Proof.
@@ -529,7 +570,6 @@ Proof.
     + contradict IHnormalized2.
       eexists.
       econstructor;eauto.
-  (* 
   - (* Sigma *)
     destruct Hnorm;subst.
     destruct K;simpl in *;inversion H2;subst.
@@ -579,9 +619,7 @@ Proof.
       * contradict H3. eauto.
     + contradict IHnormalized1;eexists;econstructor;eauto.
     + contradict IHnormalized2;eexists;econstructor;eauto.
-Admitted.
-*)
-Qed.
+Admitted. *)
 
 
 
@@ -609,8 +647,9 @@ As extra reduction step (+normalized requirement?)? As separate step in between?
 Inductive base_step : expr -> expr -> Prop :=
 (* 'real' steps (congruence steps later) *)
   | BetaS x T f U elam earg e' :
-    normalized T ->
-    is_val earg ->
+    (* not necessary if we only define beta on normalized terms *)
+    (* normalized T ->  *)
+    (* is_val earg -> *)
     e' = subst' x earg elam ->
     base_step (App (Lam x T f U elam) earg) e'
   (* | IotaTupleS es n (i:Fin.t n) e:
@@ -628,13 +667,22 @@ Inductive base_step : expr -> expr -> Prop :=
     nth_error es (` (Fin.to_nat i)) = Some e ->
     base_step (Extract (Tuple es) (LitIdx n i)) e
   (* extract of pack *)
-  | IotaPackS x e n ei e':
+  | IotaPackS x e en ei e':
     is_val ei -> (* implies ei = LitIdx n i (via canonical values?) *)
     e' = subst' x ei e ->
-    base_step (Extract (Pack x (LitNat n) e) ei) e' *)
+    (* TODO: do we need LitNat here or any arbitrary en? *)
+    (* base_step (Extract (Pack x (LitNat n) e) ei) e' *)
+    base_step (Extract (Pack x en e) ei) e' *)
   .
 
+(*
+  Extracts covered by normalization
+  for <x:en, e> # ei => e[ei/x]
+  we have a rule if en = n or x=_
+  we reach either case eventually
 
+  beta goes under binder
+*)
 
 
 (* evaluation contexts for congruence reduction *)
@@ -647,56 +695,96 @@ Inductive base_step : expr -> expr -> Prop :=
   only relevant for two sided reductions in app, extract, and tuple
 
   Note: we are a bit lazier => do not evaluate under binders
+
+
+  Change: we go under binders but not in types of dependencies => might lead to untyped code (no step in context necessary)
+  for dependent code, normalization is sufficient for our usage
 *)
 Inductive ectx :=
   | HoleCtx
   (* only context in T as U might depend on x:T *)
-  | PiCtx (x:binder) (K: ectx) (U:expr) 
+  (* | PiCtx (x:binder) (K: ectx) (U:expr)  *)
+  (* no, instead don't go under types *)
   (* the filter depends on the argument *)
-  | LamCtx (x:binder) (K: ectx) (f:expr) (U:expr) (e:expr)
+  (* | LamCtx (x:binder) (K: ectx) (f:expr) (U:expr) (e:expr) *)
+  (* do not go in (named) depency types *)
+  | LamCtx (x:binder) (T: expr) (f:expr) (U:expr) (K: ectx)
   | AppLCtx (K: ectx) (v2 : expr)
   | AppRCtx (e1 : expr) (K: ectx) (H: is_val e1)
   (* only first argument in sigma *)
-  (* | SigmaCtx (x:binder) (K: ectx) (args: list (binder * expr))
-  | TupleCtx (es1:list expr) (K: ectx) (es2: list expr) (H: Forall is_val es1)
+  (* | SigmaCtx (x:binder) (K: ectx) (args: list (binder * expr)) *)
+    (* (H: Forall is_val es1) *)
+  | TupleCtx (es1:list expr) (K: ectx) (es2: list expr) 
   (* only en is up to be a context *)
-  | ArrayCtx (x:binder) (K: ectx) (T:expr)
-  | PackCtx (x:binder) (K: ectx) (e:expr)
+  (* | ArrayCtx (x:binder) (K: ectx) (T:expr) *)
+  (* | PackCtx (x:binder) (K: ectx) (e:expr) *)
+  | PackLCtx (x:binder) (K: ectx) (e:expr)
+  | PackRCtx (x:binder) (en:expr) (K: ectx) 
   | ExtractLCtx (K: ectx) (ei:expr)
-  | ExtractRCtx (e:expr) (K: ectx) (H: is_val e) *)
+ (* (H: is_val e) *)
+  | ExtractRCtx (e:expr) (K: ectx)
+  (*
+  TODO: nothing in types? Even toplevel
+  => array, Pi, Sigma
+  *)
   .  
 
 (* Place an expression into the hole of a context *)
-Fixpoint fill (K : ectx) (e : expr) : expr :=
+(* Fixpoint fill (K : ectx) (e : expr) : expr :=
   match K with
   | HoleCtx => e
   | PiCtx x K U => Pi x (fill K e) U
-  | LamCtx x K f U eb => Lam x (fill K e) f U eb
+  (* | LamCtx x K f U eb => Lam x (fill K e) f U eb *)
   | AppLCtx K v2 => App (fill K e) v2
   | AppRCtx e1 K _ => App e1 (fill K e)
-  (* | SigmaCtx x K args => Sigma ((x, fill K e) :: args)
+  | SigmaCtx x K args => Sigma ((x, fill K e) :: args)
   | TupleCtx es1 K es2 _ => Tuple (es1 ++ fill K e :: es2)
   | ArrayCtx x K T => Array x (fill K e) T
   | PackCtx x K eb => Pack x (fill K e) eb
   | ExtractLCtx K ei => Extract (fill K e) ei
-  | ExtractRCtx eb K _ => Extract eb (fill K e) *)
+  | ExtractRCtx eb K _ => Extract eb (fill K e)
+  end. *)
+Fixpoint fill (K : ectx) (e : expr) : expr :=
+  match K with
+  | HoleCtx => e
+  | LamCtx x T f U K => Lam x T f U (fill K e)
+  | AppLCtx K v2 => App (fill K e) v2
+  | AppRCtx e1 K H => App e1 (fill K e)
+  | TupleCtx es1 K es2 => Tuple (es1 ++ fill K e :: es2)
+  | PackLCtx x K eb => Pack x (fill K e) eb
+  | PackRCtx x en K => Pack x en (fill K e)
+  | ExtractLCtx K ei => Extract (fill K e) ei
+  | ExtractRCtx eb K => Extract eb (fill K e)
   end.
 
 (* Compose two evaluation contexts => place the second context into the hole of the first *)
-Fixpoint comp_ectx (K1: ectx) (K2 : ectx) : ectx :=
+(* Fixpoint comp_ectx (K1: ectx) (K2 : ectx) : ectx :=
   match K1 with
   | HoleCtx => K2
   | PiCtx x K U => PiCtx x (comp_ectx K K2) U
-  | LamCtx x K f U e => LamCtx x (comp_ectx K K2) f U e
+  (* | LamCtx x K f U e => LamCtx x (comp_ectx K K2) f U e *)
   | AppLCtx K v2 => AppLCtx (comp_ectx K K2) v2
   | AppRCtx e1 K H => AppRCtx e1 (comp_ectx K K2) H
-  (* | SigmaCtx x K args => SigmaCtx x (comp_ectx K K2) args
+  | SigmaCtx x K args => SigmaCtx x (comp_ectx K K2) args
   | TupleCtx es1 K es2 H => TupleCtx es1 (comp_ectx K K2) es2 H
   | ArrayCtx x K T => ArrayCtx x (comp_ectx K K2) T
   | PackCtx x K e => PackCtx x (comp_ectx K K2) e
   | ExtractLCtx K ei => ExtractLCtx (comp_ectx K K2) ei
-  | ExtractRCtx e K H => ExtractRCtx e (comp_ectx K K2) H *)
+  | ExtractRCtx e K H => ExtractRCtx e (comp_ectx K K2) H
+  end. *)
+Fixpoint comp_ectx (K1: ectx) (K2 : ectx) : ectx :=
+  match K1 with
+  | HoleCtx => K2
+  | LamCtx x T f U K => LamCtx x T f U (comp_ectx K K2)
+  | AppLCtx K v2 => AppLCtx (comp_ectx K K2) v2
+  | AppRCtx e1 K H => AppRCtx e1 (comp_ectx K K2) H
+  | TupleCtx es1 K es2 => TupleCtx es1 (comp_ectx K K2) es2
+  | PackLCtx x K eb => PackLCtx x (comp_ectx K K2) eb
+  | PackRCtx x en K => PackRCtx x en (comp_ectx K K2)
+  | ExtractLCtx K ei => ExtractLCtx (comp_ectx K K2) ei
+  | ExtractRCtx eb K => ExtractRCtx eb (comp_ectx K K2)
   end.
+
 
 (** Contextual steps => lift reductions via contexts *)
 Inductive contextual_step (e1 : expr) (e2 : expr) : Prop :=
@@ -728,7 +816,6 @@ Proof.
   rewrite !fill_comp. by econstructor.
 Qed.
 
-(* TODO: we want is_val <-> ~ reducibile *)
 Lemma values_dont_reduce e:
   is_val e → ¬ reducible e.
 Proof.
@@ -743,10 +830,60 @@ Proof.
   - (* Idx #n, #n -> ... *)
     destruct K;simpl in H2;inversion H2;subst.
     inversion Hred.
-  (* - apply Forall_app in H1 as [H1 H2].
+  - apply Forall_app in H0 as [H1 H2].
     inversion H2;subst.
-    congruence. *)
+    congruence.
 Qed.
+
+
+(*
+  assume typed and normalized
+*)
+Lemma characterize_value e:
+  ¬ reducible e → is_val e.
+Proof.
+  intros H.
+  induction e;try now econstructor.
+  - admit. (* var -- ruled out by typed *)
+  - econstructor.
+    apply IHe4.
+    contradict H.
+    destruct H as [ebody' H].
+    destruct H as [K e1' e2' -> -> Hred].
+    eexists. 
+    eapply Ectx_step with (K:=LamCtx x e1 e2 e3 K);eauto.
+  - contradict H.
+    (* app *)
+    (* if typed and normalized => lambda => makes an app step *)
+    admit.
+  - admit. (* nested induction *)
+  - (* pack *)
+    admit.
+  - (* extract *)
+    (* if normalized (and typed), all extracts are evaluated *)
+    admit.
+Abort.
+
+
+(* TODO: we want is_val <-> ~ reducibile *)
+(* Lemma values_dont_reduce e:
+  is_val e → ¬ reducible e.
+Proof.
+  intros Hv Hred.
+  destruct Hred.
+  destruct H as [K e1 e2 -> -> Hred].
+  induction K;simpl in Hv;inversion Hv;subst;try congruence.
+  all: try (now inversion Hred).
+  - (* Idx #n, Idx -> ... *)
+    destruct K;simpl in *;inversion H0;subst.
+    inversion Hred.
+  - (* Idx #n, #n -> ... *)
+    destruct K;simpl in H2;inversion H2;subst.
+    inversion Hred.
+  - apply Forall_app in H1 as [H1 H2].
+    inversion H2;subst.
+    congruence.
+Qed. *)
 
 (*
 lemma is_val -> normalized
@@ -790,12 +927,12 @@ Abort. *)
   e#0_1 -> e
   use canonical values => tuple/pack
 *)
-(* Lemma norm_red e e':
+Lemma norm_red e e':
     normalize_step e e' → base_step e e'.
 Proof.
   intros Hnorm.
   inversion Hnorm;subst.
-Abort. *)
+Abort.
 
 (* TODO: not necessarily: the redex might be under a binder *)
 (* Lemma normalizable_reducible e:
@@ -902,7 +1039,7 @@ we need these lemmas for progress
 however, the context is an indirection over a simplification requiring a lemma to ease the automation burdon
 *)
 
-Lemma contextual_step_pi x T U T':
+(* Lemma contextual_step_pi x T U T':
   contextual_step T T' →
   contextual_step (Pi x T U) (Pi x T' U).
 Proof.
@@ -910,13 +1047,13 @@ Proof.
   by eapply (fill_contextual_step (PiCtx x HoleCtx U)).
 Qed.
 
-Lemma contextual_step_lam x ef U e T T':
+(* Lemma contextual_step_lam x ef U e T T':
   contextual_step T T' →
   contextual_step (Lam x T ef U e) (Lam x T' ef U e).
 Proof.
   intros Hcontextual.
   by eapply (fill_contextual_step (LamCtx x HoleCtx ef U e)).
-Qed.
+Qed. *)
 
 Lemma contextual_step_app_l e1 e1' e2:
   contextual_step e1 e1' →
@@ -935,7 +1072,7 @@ Proof.
   by apply (fill_contextual_step (AppRCtx e1 HoleCtx H)).
 Qed.
 
-(* Lemma contextual_step_sigma x T T' xs:
+Lemma contextual_step_sigma x T T' xs:
   contextual_step T T' →
   contextual_step (Sigma ((x, T) :: xs)) (Sigma ((x, T') :: xs)).
 Proof.
@@ -983,21 +1120,21 @@ Lemma contextual_step_extract_r e ei ei':
 Proof.
   intros H Hcontextual.
   by apply (fill_contextual_step (ExtractRCtx e HoleCtx H)).
-Qed. *)
+Qed.
 
 #[export]
 Hint Resolve
   contextual_step_pi
-  contextual_step_lam
+  (* contextual_step_lam *)
   contextual_step_app_l
   contextual_step_app_r
-  (* contextual_step_sigma
+  contextual_step_sigma
   contextual_step_tuple
   contextual_step_array
   contextual_step_pack
   contextual_step_extract_l
-  contextual_step_extract_r *)
+  contextual_step_extract_r
   : core.
 
 
-
+ *)
