thorin/smt/lam.smt2
@@ -1,0 +1,33 @@
+(set-logic ALL)
+; (set-logic AUFNIRA)
+; (set-logic QF_LIA)
+
+; smt2 definition of lambda calculus type
+(declare-datatypes ((Typ 0)) (((Unit) (Arrow (arg Typ) (res Typ)))))
+; now expressions
+(declare-datatypes ((Exp 0)) (((Var (index Int)) (Abs (body Exp)) (App (fun Exp) (arg Exp)) (One))))
+
+; (assert true)
+; (declare-fun typed (Exp Typ) Bool)
+; with environment
+(declare-fun typed ((Array Int Typ) Exp Typ) Bool)
+
+; x : A |- x : A
+(assert (forall ((env (Array Int Typ)) (i Int) (A Typ))
+  (=> 
+    (= A (select env i))
+    (typed env (Var i) A)
+  )
+))
+
+; |- One : Unit
+(assert (forall ((env (Array Int Typ)))
+  (typed env One (Unit))
+))
+    
+(declare-const e Exp)
+; (assert (not (exists ((env (Array Int Typ)) (A Typ)) (typed env e A))))
+(assert (forall ((env (Array Int Typ)) (A Typ)) (not (typed env e A))))
+
+(check-sat)
+(get-model)
